libcrux-ml-dsa/proofs/fstar/extraction/Libcrux_ml_dsa.Ml_dsa_generic.Instantiations.Neon.Ml_dsa_87_.fst
@@ -1,0 +1,115 @@
+module Libcrux_ml_dsa.Ml_dsa_generic.Instantiations.Neon.Ml_dsa_87_
+#set-options "--fuel 0 --ifuel 1 --z3rlimit 100"
+open Core
+open FStar.Mul
+
+let _ =
+  (* This module has implicit dependencies, here we make them explicit. *)
+  (* The implicit dependencies arise from typeclasses instances. *)
+  let open Libcrux_ml_dsa.Hash_functions.Neon in
+  let open Libcrux_ml_dsa.Hash_functions.Portable in
+  let open Libcrux_ml_dsa.Hash_functions.Shake128 in
+  let open Libcrux_ml_dsa.Hash_functions.Shake256 in
+  let open Libcrux_ml_dsa.Pre_hash in
+  let open Libcrux_ml_dsa.Samplex4 in
+  let open Libcrux_ml_dsa.Samplex4.Neon in
+  let open Libcrux_ml_dsa.Simd.Portable in
+  let open Libcrux_ml_dsa.Simd.Traits in
+  ()
+
+let generate_key_pair
+      (randomness: t_Array u8 (sz 32))
+      (signing_key: t_Array u8 (sz 4896))
+      (verification_key: t_Array u8 (sz 2592))
+     =
+  let tmp0, tmp1:(t_Array u8 (sz 4896) & t_Array u8 (sz 2592)) =
+    Libcrux_ml_dsa.Ml_dsa_generic.Ml_dsa_87_.generate_key_pair #Libcrux_ml_dsa.Simd.Portable.Vector_type.t_PortableSIMDUnit
+      #Libcrux_ml_dsa.Samplex4.Neon.t_NeonSampler
+      #Libcrux_ml_dsa.Hash_functions.Neon.t_Shake128x4
+      #Libcrux_ml_dsa.Hash_functions.Portable.t_Shake256
+      #Libcrux_ml_dsa.Hash_functions.Portable.t_Shake256Xof
+      #Libcrux_ml_dsa.Hash_functions.Neon.t_Shake256x4
+      randomness
+      signing_key
+      verification_key
+  in
+  let signing_key:t_Array u8 (sz 4896) = tmp0 in
+  let verification_key:t_Array u8 (sz 2592) = tmp1 in
+  let hax_temp_output:Prims.unit = () in
+  signing_key, verification_key <: (t_Array u8 (sz 4896) & t_Array u8 (sz 2592))
+
+let sign
+      (signing_key: t_Array u8 (sz 4896))
+      (message context: t_Slice u8)
+      (randomness: t_Array u8 (sz 32))
+     =
+  Libcrux_ml_dsa.Ml_dsa_generic.Ml_dsa_87_.sign #Libcrux_ml_dsa.Simd.Portable.Vector_type.t_PortableSIMDUnit
+    #Libcrux_ml_dsa.Samplex4.Neon.t_NeonSampler #Libcrux_ml_dsa.Hash_functions.Neon.t_Shake128x4
+    #Libcrux_ml_dsa.Hash_functions.Portable.t_Shake256
+    #Libcrux_ml_dsa.Hash_functions.Portable.t_Shake256Xof
+    #Libcrux_ml_dsa.Hash_functions.Neon.t_Shake256x4 (signing_key <: t_Slice u8) message context
+    randomness
+
+let sign_pre_hashed_shake128
+      (signing_key: t_Array u8 (sz 4896))
+      (message context pre_hash_buffer: t_Slice u8)
+      (randomness: t_Array u8 (sz 32))
+     =
+  let tmp0, out:(t_Slice u8 &
+    Core.Result.t_Result (Libcrux_ml_dsa.Types.t_MLDSASignature (sz 4627))
+      Libcrux_ml_dsa.Types.t_SigningError) =
+    Libcrux_ml_dsa.Ml_dsa_generic.Ml_dsa_87_.sign_pre_hashed #Libcrux_ml_dsa.Simd.Portable.Vector_type.t_PortableSIMDUnit
+      #Libcrux_ml_dsa.Samplex4.Neon.t_NeonSampler #Libcrux_ml_dsa.Hash_functions.Portable.t_Shake128
+      #Libcrux_ml_dsa.Hash_functions.Neon.t_Shake128x4
+      #Libcrux_ml_dsa.Hash_functions.Portable.t_Shake256
+      #Libcrux_ml_dsa.Hash_functions.Portable.t_Shake256Xof
+      #Libcrux_ml_dsa.Hash_functions.Neon.t_Shake256x4 #Libcrux_ml_dsa.Pre_hash.t_SHAKE128_PH
+      (signing_key <: t_Slice u8) message context pre_hash_buffer randomness
+  in
+  let pre_hash_buffer:t_Slice u8 = tmp0 in
+  let hax_temp_output:Core.Result.t_Result (Libcrux_ml_dsa.Types.t_MLDSASignature (sz 4627))
+    Libcrux_ml_dsa.Types.t_SigningError =
+    out
+  in
+  pre_hash_buffer, hax_temp_output
+  <:
+  (t_Slice u8 &
+    Core.Result.t_Result (Libcrux_ml_dsa.Types.t_MLDSASignature (sz 4627))
+      Libcrux_ml_dsa.Types.t_SigningError)
+
+let verify
+      (verification_key: t_Array u8 (sz 2592))
+      (message context: t_Slice u8)
+      (signature: t_Array u8 (sz 4627))
+     =
+  Libcrux_ml_dsa.Ml_dsa_generic.Ml_dsa_87_.verify #Libcrux_ml_dsa.Simd.Portable.Vector_type.t_PortableSIMDUnit
+    #Libcrux_ml_dsa.Samplex4.Neon.t_NeonSampler
+    #Libcrux_ml_dsa.Hash_functions.Neon.t_Shake128x4
+    #Libcrux_ml_dsa.Hash_functions.Portable.t_Shake256
+    #Libcrux_ml_dsa.Hash_functions.Portable.t_Shake256Xof
+    verification_key
+    message
+    context
+    signature
+
+let verify_pre_hashed_shake128
+      (verification_key: t_Array u8 (sz 2592))
+      (message context pre_hash_buffer: t_Slice u8)
+      (signature: t_Array u8 (sz 4627))
+     =
+  let tmp0, out:(t_Slice u8 &
+    Core.Result.t_Result Prims.unit Libcrux_ml_dsa.Types.t_VerificationError) =
+    Libcrux_ml_dsa.Ml_dsa_generic.Ml_dsa_87_.verify_pre_hashed #Libcrux_ml_dsa.Simd.Portable.Vector_type.t_PortableSIMDUnit
+      #Libcrux_ml_dsa.Samplex4.Neon.t_NeonSampler #Libcrux_ml_dsa.Hash_functions.Portable.t_Shake128
+      #Libcrux_ml_dsa.Hash_functions.Neon.t_Shake128x4
+      #Libcrux_ml_dsa.Hash_functions.Portable.t_Shake256
+      #Libcrux_ml_dsa.Hash_functions.Portable.t_Shake256Xof #Libcrux_ml_dsa.Pre_hash.t_SHAKE128_PH
+      verification_key message context pre_hash_buffer signature
+  in
+  let pre_hash_buffer:t_Slice u8 = tmp0 in
+  let hax_temp_output:Core.Result.t_Result Prims.unit Libcrux_ml_dsa.Types.t_VerificationError =
+    out
+  in
+  pre_hash_buffer, hax_temp_output
+  <:
+  (t_Slice u8 & Core.Result.t_Result Prims.unit Libcrux_ml_dsa.Types.t_VerificationError)
