libcrux-ml-dsa/proofs/fstar/extraction/Libcrux_ml_dsa.Ml_dsa_generic.Ml_dsa_87_.fsti
@@ -1,0 +1,165 @@
+module Libcrux_ml_dsa.Ml_dsa_generic.Ml_dsa_87_
+#set-options "--fuel 0 --ifuel 1 --z3rlimit 100"
+open Core
+open FStar.Mul
+
+let _ =
+  (* This module has implicit dependencies, here we make them explicit. *)
+  (* The implicit dependencies arise from typeclasses instances. *)
+  let open Libcrux_ml_dsa.Hash_functions.Shake128 in
+  let open Libcrux_ml_dsa.Hash_functions.Shake256 in
+  let open Libcrux_ml_dsa.Polynomial in
+  let open Libcrux_ml_dsa.Pre_hash in
+  let open Libcrux_ml_dsa.Samplex4 in
+  let open Libcrux_ml_dsa.Simd.Traits in
+  ()
+
+let v_BETA: i32 =
+  Libcrux_ml_dsa.Constants.beta Libcrux_ml_dsa.Constants.Ml_dsa_87_.v_ONES_IN_VERIFIER_CHALLENGE
+    Libcrux_ml_dsa.Constants.Ml_dsa_87_.v_ETA
+
+let v_COMMITMENT_RING_ELEMENT_SIZE: usize =
+  Libcrux_ml_dsa.Constants.commitment_ring_element_size Libcrux_ml_dsa.Constants.Ml_dsa_87_.v_BITS_PER_COMMITMENT_COEFFICIENT
+
+let v_COMMITMENT_VECTOR_SIZE: usize =
+  Libcrux_ml_dsa.Constants.commitment_vector_size Libcrux_ml_dsa.Constants.Ml_dsa_87_.v_BITS_PER_COMMITMENT_COEFFICIENT
+    Libcrux_ml_dsa.Constants.Ml_dsa_87_.v_ROWS_IN_A
+
+let v_ERROR_RING_ELEMENT_SIZE: usize =
+  Libcrux_ml_dsa.Constants.error_ring_element_size Libcrux_ml_dsa.Constants.Ml_dsa_87_.v_BITS_PER_ERROR_COEFFICIENT
+
+let v_GAMMA1_RING_ELEMENT_SIZE: usize =
+  Libcrux_ml_dsa.Constants.gamma1_ring_element_size Libcrux_ml_dsa.Constants.Ml_dsa_87_.v_BITS_PER_GAMMA1_COEFFICIENT
+
+let v_ROW_COLUMN: usize =
+  Libcrux_ml_dsa.Constants.Ml_dsa_87_.v_ROWS_IN_A +!
+  Libcrux_ml_dsa.Constants.Ml_dsa_87_.v_COLUMNS_IN_A
+
+let v_ROW_X_COLUMN: usize =
+  Libcrux_ml_dsa.Constants.Ml_dsa_87_.v_ROWS_IN_A *!
+  Libcrux_ml_dsa.Constants.Ml_dsa_87_.v_COLUMNS_IN_A
+
+let v_SIGNATURE_SIZE: usize =
+  Libcrux_ml_dsa.Constants.signature_size Libcrux_ml_dsa.Constants.Ml_dsa_87_.v_ROWS_IN_A
+    Libcrux_ml_dsa.Constants.Ml_dsa_87_.v_COLUMNS_IN_A
+    Libcrux_ml_dsa.Constants.Ml_dsa_87_.v_MAX_ONES_IN_HINT
+    Libcrux_ml_dsa.Constants.Ml_dsa_87_.v_COMMITMENT_HASH_SIZE
+    Libcrux_ml_dsa.Constants.Ml_dsa_87_.v_BITS_PER_GAMMA1_COEFFICIENT
+
+let v_SIGNING_KEY_SIZE: usize =
+  Libcrux_ml_dsa.Constants.signing_key_size Libcrux_ml_dsa.Constants.Ml_dsa_87_.v_ROWS_IN_A
+    Libcrux_ml_dsa.Constants.Ml_dsa_87_.v_COLUMNS_IN_A
+    v_ERROR_RING_ELEMENT_SIZE
+
+let v_VERIFICATION_KEY_SIZE: usize =
+  Libcrux_ml_dsa.Constants.verification_key_size Libcrux_ml_dsa.Constants.Ml_dsa_87_.v_ROWS_IN_A
+
+val sign_internal
+      (#v_SIMDUnit #v_Sampler #v_Shake128X4 #v_Shake256 #v_Shake256Xof #v_Shake256X4: Type0)
+      {| i6: Libcrux_ml_dsa.Simd.Traits.t_Operations v_SIMDUnit |}
+      {| i7: Libcrux_ml_dsa.Samplex4.t_X4Sampler v_Sampler |}
+      {| i8: Libcrux_ml_dsa.Hash_functions.Shake128.t_XofX4 v_Shake128X4 |}
+      {| i9: Libcrux_ml_dsa.Hash_functions.Shake256.t_DsaXof v_Shake256 |}
+      {| i10: Libcrux_ml_dsa.Hash_functions.Shake256.t_Xof v_Shake256Xof |}
+      {| i11: Libcrux_ml_dsa.Hash_functions.Shake256.t_XofX4 v_Shake256X4 |}
+      (signing_key message: t_Slice u8)
+      (domain_separation_context:
+          Core.Option.t_Option Libcrux_ml_dsa.Pre_hash.t_DomainSeparationContext)
+      (randomness: t_Array u8 (sz 32))
+    : Prims.Pure
+      (Core.Result.t_Result (Libcrux_ml_dsa.Types.t_MLDSASignature (sz 4627))
+          Libcrux_ml_dsa.Types.t_SigningError) Prims.l_True (fun _ -> Prims.l_True)
+
+val sign
+      (#v_SIMDUnit #v_Sampler #v_Shake128X4 #v_Shake256 #v_Shake256Xof #v_Shake256X4: Type0)
+      {| i6: Libcrux_ml_dsa.Simd.Traits.t_Operations v_SIMDUnit |}
+      {| i7: Libcrux_ml_dsa.Samplex4.t_X4Sampler v_Sampler |}
+      {| i8: Libcrux_ml_dsa.Hash_functions.Shake128.t_XofX4 v_Shake128X4 |}
+      {| i9: Libcrux_ml_dsa.Hash_functions.Shake256.t_DsaXof v_Shake256 |}
+      {| i10: Libcrux_ml_dsa.Hash_functions.Shake256.t_Xof v_Shake256Xof |}
+      {| i11: Libcrux_ml_dsa.Hash_functions.Shake256.t_XofX4 v_Shake256X4 |}
+      (signing_key message context: t_Slice u8)
+      (randomness: t_Array u8 (sz 32))
+    : Prims.Pure
+      (Core.Result.t_Result (Libcrux_ml_dsa.Types.t_MLDSASignature (sz 4627))
+          Libcrux_ml_dsa.Types.t_SigningError) Prims.l_True (fun _ -> Prims.l_True)
+
+val sign_pre_hashed
+      (#v_SIMDUnit #v_Sampler #v_Shake128 #v_Shake128X4 #v_Shake256 #v_Shake256Xof #v_Shake256X4 #v_PH:
+          Type0)
+      {| i8: Libcrux_ml_dsa.Simd.Traits.t_Operations v_SIMDUnit |}
+      {| i9: Libcrux_ml_dsa.Samplex4.t_X4Sampler v_Sampler |}
+      {| i10: Libcrux_ml_dsa.Hash_functions.Shake128.t_Xof v_Shake128 |}
+      {| i11: Libcrux_ml_dsa.Hash_functions.Shake128.t_XofX4 v_Shake128X4 |}
+      {| i12: Libcrux_ml_dsa.Hash_functions.Shake256.t_DsaXof v_Shake256 |}
+      {| i13: Libcrux_ml_dsa.Hash_functions.Shake256.t_Xof v_Shake256Xof |}
+      {| i14: Libcrux_ml_dsa.Hash_functions.Shake256.t_XofX4 v_Shake256X4 |}
+      {| i15: Libcrux_ml_dsa.Pre_hash.t_PreHash v_PH |}
+      (signing_key message context pre_hash_buffer: t_Slice u8)
+      (randomness: t_Array u8 (sz 32))
+    : Prims.Pure
+      (t_Slice u8 &
+        Core.Result.t_Result (Libcrux_ml_dsa.Types.t_MLDSASignature (sz 4627))
+          Libcrux_ml_dsa.Types.t_SigningError) Prims.l_True (fun _ -> Prims.l_True)
+
+/// The internal verification API.
+/// If no `domain_separation_context` is supplied, it is assumed that
+/// `message` already contains the domain separation.
+val verify_internal
+      (#v_SIMDUnit #v_Sampler #v_Shake128X4 #v_Shake256 #v_Shake256Xof: Type0)
+      {| i5: Libcrux_ml_dsa.Simd.Traits.t_Operations v_SIMDUnit |}
+      {| i6: Libcrux_ml_dsa.Samplex4.t_X4Sampler v_Sampler |}
+      {| i7: Libcrux_ml_dsa.Hash_functions.Shake128.t_XofX4 v_Shake128X4 |}
+      {| i8: Libcrux_ml_dsa.Hash_functions.Shake256.t_DsaXof v_Shake256 |}
+      {| i9: Libcrux_ml_dsa.Hash_functions.Shake256.t_Xof v_Shake256Xof |}
+      (verification_key: t_Array u8 (sz 2592))
+      (message: t_Slice u8)
+      (domain_separation_context:
+          Core.Option.t_Option Libcrux_ml_dsa.Pre_hash.t_DomainSeparationContext)
+      (signature_serialized: t_Array u8 (sz 4627))
+    : Prims.Pure (Core.Result.t_Result Prims.unit Libcrux_ml_dsa.Types.t_VerificationError)
+      Prims.l_True
+      (fun _ -> Prims.l_True)
+
+val verify
+      (#v_SIMDUnit #v_Sampler #v_Shake128X4 #v_Shake256 #v_Shake256Xof: Type0)
+      {| i5: Libcrux_ml_dsa.Simd.Traits.t_Operations v_SIMDUnit |}
+      {| i6: Libcrux_ml_dsa.Samplex4.t_X4Sampler v_Sampler |}
+      {| i7: Libcrux_ml_dsa.Hash_functions.Shake128.t_XofX4 v_Shake128X4 |}
+      {| i8: Libcrux_ml_dsa.Hash_functions.Shake256.t_DsaXof v_Shake256 |}
+      {| i9: Libcrux_ml_dsa.Hash_functions.Shake256.t_Xof v_Shake256Xof |}
+      (verification_key_serialized: t_Array u8 (sz 2592))
+      (message context: t_Slice u8)
+      (signature_serialized: t_Array u8 (sz 4627))
+    : Prims.Pure (Core.Result.t_Result Prims.unit Libcrux_ml_dsa.Types.t_VerificationError)
+      Prims.l_True
+      (fun _ -> Prims.l_True)
+
+val verify_pre_hashed
+      (#v_SIMDUnit #v_Sampler #v_Shake128 #v_Shake128X4 #v_Shake256 #v_Shake256Xof #v_PH: Type0)
+      {| i7: Libcrux_ml_dsa.Simd.Traits.t_Operations v_SIMDUnit |}
+      {| i8: Libcrux_ml_dsa.Samplex4.t_X4Sampler v_Sampler |}
+      {| i9: Libcrux_ml_dsa.Hash_functions.Shake128.t_Xof v_Shake128 |}
+      {| i10: Libcrux_ml_dsa.Hash_functions.Shake128.t_XofX4 v_Shake128X4 |}
+      {| i11: Libcrux_ml_dsa.Hash_functions.Shake256.t_DsaXof v_Shake256 |}
+      {| i12: Libcrux_ml_dsa.Hash_functions.Shake256.t_Xof v_Shake256Xof |}
+      {| i13: Libcrux_ml_dsa.Pre_hash.t_PreHash v_PH |}
+      (verification_key_serialized: t_Array u8 (sz 2592))
+      (message context pre_hash_buffer: t_Slice u8)
+      (signature_serialized: t_Array u8 (sz 4627))
+    : Prims.Pure
+      (t_Slice u8 & Core.Result.t_Result Prims.unit Libcrux_ml_dsa.Types.t_VerificationError)
+      Prims.l_True
+      (fun _ -> Prims.l_True)
+
+val generate_key_pair
+      (#v_SIMDUnit #v_Sampler #v_Shake128X4 #v_Shake256 #v_Shake256Xof #v_Shake256X4: Type0)
+      {| i6: Libcrux_ml_dsa.Simd.Traits.t_Operations v_SIMDUnit |}
+      {| i7: Libcrux_ml_dsa.Samplex4.t_X4Sampler v_Sampler |}
+      {| i8: Libcrux_ml_dsa.Hash_functions.Shake128.t_XofX4 v_Shake128X4 |}
+      {| i9: Libcrux_ml_dsa.Hash_functions.Shake256.t_DsaXof v_Shake256 |}
+      {| i10: Libcrux_ml_dsa.Hash_functions.Shake256.t_Xof v_Shake256Xof |}
+      {| i11: Libcrux_ml_dsa.Hash_functions.Shake256.t_XofX4 v_Shake256X4 |}
+      (randomness: t_Array u8 (sz 32))
+      (signing_key verification_key: t_Slice u8)
+    : Prims.Pure (t_Slice u8 & t_Slice u8) Prims.l_True (fun _ -> Prims.l_True)
