libcrux-ml-dsa/proofs/fstar/extraction/Libcrux_ml_dsa.Ml_dsa_generic.Multiplexing.Ml_dsa_65_.fsti
@@ -1,0 +1,44 @@
+module Libcrux_ml_dsa.Ml_dsa_generic.Multiplexing.Ml_dsa_65_
+#set-options "--fuel 0 --ifuel 1 --z3rlimit 100"
+open Core
+open FStar.Mul
+
+val generate_key_pair
+      (randomness: t_Array u8 (sz 32))
+      (signing_key: t_Array u8 (sz 4032))
+      (verification_key: t_Array u8 (sz 1952))
+    : Prims.Pure (t_Array u8 (sz 4032) & t_Array u8 (sz 1952)) Prims.l_True (fun _ -> Prims.l_True)
+
+val sign
+      (signing_key: t_Array u8 (sz 4032))
+      (message context: t_Slice u8)
+      (randomness: t_Array u8 (sz 32))
+    : Prims.Pure
+      (Core.Result.t_Result (Libcrux_ml_dsa.Types.t_MLDSASignature (sz 3309))
+          Libcrux_ml_dsa.Types.t_SigningError) Prims.l_True (fun _ -> Prims.l_True)
+
+val sign_pre_hashed_shake128
+      (signing_key: t_Array u8 (sz 4032))
+      (message context pre_hash_buffer: t_Slice u8)
+      (randomness: t_Array u8 (sz 32))
+    : Prims.Pure
+      (t_Slice u8 &
+        Core.Result.t_Result (Libcrux_ml_dsa.Types.t_MLDSASignature (sz 3309))
+          Libcrux_ml_dsa.Types.t_SigningError) Prims.l_True (fun _ -> Prims.l_True)
+
+val verify
+      (verification_key_serialized: t_Array u8 (sz 1952))
+      (message context: t_Slice u8)
+      (signature_serialized: t_Array u8 (sz 3309))
+    : Prims.Pure (Core.Result.t_Result Prims.unit Libcrux_ml_dsa.Types.t_VerificationError)
+      Prims.l_True
+      (fun _ -> Prims.l_True)
+
+val verify_pre_hashed_shake128
+      (verification_key_serialized: t_Array u8 (sz 1952))
+      (message context pre_hash_buffer: t_Slice u8)
+      (signature_serialized: t_Array u8 (sz 3309))
+    : Prims.Pure
+      (t_Slice u8 & Core.Result.t_Result Prims.unit Libcrux_ml_dsa.Types.t_VerificationError)
+      Prims.l_True
+      (fun _ -> Prims.l_True)
